{"cells":[{"cell_type":"markdown","metadata":{},"source":["# 5. The Predicate Calculus"]},{"cell_type":"code","execution_count":1,"metadata":{},"outputs":[],"source":["import re\n","\n","from itertools import product\n","from sympy import (\n","    false,\n","    true\n",")\n","from sympy.abc import *\n","from sympy.logic.boolalg import Equivalent"]},{"cell_type":"code","execution_count":2,"metadata":{},"outputs":[],"source":["def logic_table(expr):\n","    \"\"\" Pass a function to test all logical results. \"\"\"\n","    args = expr.atoms()\n","    for prod in product((true, false), repeat = len(args)):\n","        expr_str = expr\n","        for x in zip(args, prod):\n","            target = r\"\\b\" + str(x[0]) + r\"\\b\"\n","            replace = str(x[1])\n","            expr_str = re.sub(target, replace, str(expr_str))\n","        result = str(expr.subs(zip(args, prod)))\n","        print(str(expr_str) + \" = \" + result)"]},{"cell_type":"code","execution_count":3,"metadata":{},"outputs":[{"name":"stdout","output_type":"stream","text":["True = True\n","False = False\n"]}],"source":["def F(x):\n","    return ~x\n","\n","def G(x):\n","    return ~~x\n","\n","tautology = (F(x) >> G(x)) >> (~G(x) >> ~F(x))\n","logic_table(tautology)"]},{"cell_type":"code","execution_count":4,"metadata":{},"outputs":[{"name":"stdout","output_type":"stream","text":["True = True\n","False = False\n"]}],"source":["tautology = Equivalent(F(x), ~~F(x))\n","logic_table(tautology)"]},{"cell_type":"markdown","metadata":{},"source":[" > A *formal proof* in a predicate language is a finite sequence of formulas of that language in which each formula is either an axiom or results from prior formulas of the sequence by one of the rules of inference."]},{"cell_type":"markdown","metadata":{},"source":[" The axioms are:\n","\n"," i. All tautologies of the language\n","\n"," ii. For each term $t$ and for each formula $F(x)$ with a free variable, all formulas of either of the forms:\n","\n"," $$\n"," ((\\forall x)F(x)) \\implies F(t), F(t) \\implies (\\exists x)F(x)\n"," $$"]},{"cell_type":"markdown","metadata":{},"source":[" The rules of inference are:\n","\n"," iii. Modus Ponens: From $F$ and $F \\implies G$ infer $G$\n","\n"," iv. Generalization; if the variable $x$ does not occur free in $F$:\n","\n"," iv.a. From $F \\implies G(x)$ infer $F \\implies (\\forall x) G(x)$\n","\n"," iv.b From $G(x) \\implies F$ infer $((\\exists x) G(x)) \\implies F$"]}],"metadata":{"interpreter":{"hash":"5c36988f6934d5f298e2ed50ec8ee55dd622f2d2c8c2fffd8d1cfcc03df05c4a"},"kernelspec":{"display_name":"Python 3.7.6 64-bit ('general': venv)","language":"python","name":"python3"},"language_info":{"codemirror_mode":{"name":"ipython","version":3},"file_extension":".py","mimetype":"text/x-python","name":"python","nbconvert_exporter":"python","pygments_lexer":"ipython3","version":"3.7.6"},"orig_nbformat":4},"nbformat":4,"nbformat_minor":2}
